theories/operations.v
@@ -677,6 +677,8 @@ Definition those_const_list (es : list administrative_instruction) : option (lis
 
 (** Store extensions **)
 
+(* Min limit can only grow (component can only grow) &
+   Max limit remains invariant *)
 Definition limits_extension (l1 l2: limits) :=
   (l1.(lim_min) <= l2.(lim_min)) &&
   (l1.(lim_max) == l2.(lim_max)).
